Unsigned.thy
@@ -1,14 +1,14 @@
 theory Unsigned
-  imports Main HOL.Nat "HOL-Library.Monad_Syntax"
+  imports Main HOL.Nat "Word_Lib.Word_64" "Word_Lib.Word_8" Cont_Monad_Algebra
 begin
 
-datatype u8 = u8 nat
-datatype u64 = u64 nat
+type_synonym u8 = "8 word"
+type_synonym u64 = "64 word"
 datatype Slot = Slot u64
 datatype Epoch = Epoch u64
 
-primrec u64_to_nat :: "u64 \<Rightarrow> nat" where
-  "u64_to_nat (u64 n) = n"
+abbreviation u64_to_nat :: "u64 \<Rightarrow> nat" where
+  "u64_to_nat \<equiv> Word.the_nat"
 
 primrec slot_to_u64 :: "Slot \<Rightarrow> u64" where
   "slot_to_u64 (Slot n) = n"
@@ -16,37 +16,19 @@ primrec slot_to_u64 :: "Slot \<Rightarrow> u64" where
 primrec epoch_to_u64 :: "Epoch \<Rightarrow> u64" where
   "epoch_to_u64 (Epoch n) = n"
 
-definition valid_u64 :: "u64 \<Rightarrow> bool" where
-  "valid_u64 n \<equiv> u64_to_nat n < 2 ^ 64"
-
-definition valid_slot :: "Slot \<Rightarrow> bool" where
-  "valid_slot s \<equiv> valid_u64 (slot_to_u64 s)"
-
-definition valid_epoch :: "Epoch \<Rightarrow> bool" where
-  "valid_epoch e \<equiv> valid_u64 (epoch_to_u64 e)"
+lemma u64_upper_bound: "u64_to_nat x < 2 ^ 64"
+  apply (rule Orderings.xtrans(1)[where b="2 ^ LENGTH(64)"])
+   apply force
+  by (metis nat_less_numeral_power_cancel_iff take_bit_int_less_exp the_nat.rep_eq)
 
 lemma u64_to_nat_bij: "(u64_to_nat x = u64_to_nat y) = (x = y)"
-  by (case_tac x; case_tac y; auto)
+  by auto
 
 lemma slot_to_u64_bij: "(slot_to_u64 x = slot_to_u64 y) = (x = y)"
   by (case_tac x; case_tac y; auto)
 
 lemma epoch_to_u64_bij: "(epoch_to_u64 x = epoch_to_u64 y) = (x = y)"
   by (case_tac x; case_tac y; auto)
-
-(* Linear order instance for u64 *)
-instantiation u64 :: linorder
-begin
-
-definition less_eq_u64 :: "u64 \<Rightarrow> u64 \<Rightarrow> bool" where
-  "less_eq_u64 x y \<equiv> u64_to_nat x \<le> u64_to_nat y"
-
-definition less_u64 :: "u64 \<Rightarrow> u64 \<Rightarrow> bool" where
-  "less_u64 x y \<equiv> u64_to_nat x < u64_to_nat y"
-
-instance
-  by (intro_classes; auto simp: less_eq_u64_def less_u64_def u64_to_nat_bij)
-end
 
 (* Linear order instance for Slot *)
 instantiation Slot :: linorder
@@ -77,132 +59,5 @@ instance
   by (intro_classes;
       auto intro: order_neq_le_trans simp: less_eq_Epoch_def less_Epoch_def epoch_to_u64_bij)
 end
-
-(* Unsigned arithmetic operators with overflow checks *)
-consts
-  unsigned_add :: "'a \<Rightarrow> 'a \<Rightarrow> 'a option"
-  unsigned_sub :: "'a \<Rightarrow> 'a \<Rightarrow> 'a option"
-  unsigned_mul :: "'a \<Rightarrow> 'a \<Rightarrow> 'a option"
-  unsigned_div :: "'a \<Rightarrow> 'a \<Rightarrow> 'a option"
-  unsigned_mod :: "'a \<Rightarrow> 'a \<Rightarrow> 'a option"
-
-notation
-  unsigned_add (infixl ".+" 65) and
-  unsigned_sub (infixl ".-" 65) and
-  unsigned_mul (infixl ".*" 70) and
-  unsigned_div (infixl "\\" 70) and
-  unsigned_mod (infixl ".%" 75)
-
-definition check_bin_op_then ::
-  "('a \<Rightarrow> 'b) \<Rightarrow>
-   ('b \<Rightarrow> 'a) \<Rightarrow>
-   ('a \<Rightarrow> 'a \<Rightarrow> bool) \<Rightarrow>
-   ('a \<Rightarrow> bool) \<Rightarrow>
-   ('b \<Rightarrow> 'b \<Rightarrow> 'b option) \<Rightarrow>
-   'a \<Rightarrow> 'a \<Rightarrow> 'a option" where
-  "check_bin_op_then unwrap wrap arg_check check op x y \<equiv>
-    if arg_check x y then do {
-      result_b \<leftarrow> op (unwrap x) (unwrap y);
-      let result_a = wrap result_b;
-      if check result_a then Some result_a else None
-    } else None"
-
-definition check_bin_op ::
-  "('a \<Rightarrow> 'b) \<Rightarrow>
-   ('b \<Rightarrow> 'a) \<Rightarrow>
-   ('a \<Rightarrow> 'a \<Rightarrow> bool) \<Rightarrow>
-   ('a \<Rightarrow> bool) \<Rightarrow>
-   ('b \<Rightarrow> 'b \<Rightarrow> 'b) \<Rightarrow>
-   'a \<Rightarrow> 'a \<Rightarrow> 'a option" where
-  "check_bin_op unwrap wrap arg_check check op \<equiv>
-    check_bin_op_then unwrap wrap arg_check check (\<lambda>x y. Some (op x y))"
-
-definition any_args :: "'a \<Rightarrow> 'a \<Rightarrow> bool" where
-  "any_args _ _ \<equiv> True"
-
-definition u64_add :: "u64 \<Rightarrow> u64 \<Rightarrow> u64 option" where
-  "u64_add \<equiv> check_bin_op u64_to_nat u64 any_args valid_u64 (+)"
-
-definition u64_sub :: "u64 \<Rightarrow> u64 \<Rightarrow> u64 option" where
-  "u64_sub \<equiv>
-    check_bin_op u64_to_nat u64 (\<lambda>x y. u64_to_nat x \<ge> u64_to_nat y) valid_u64 (-)"
-
-definition u64_mul :: "u64 \<Rightarrow> u64 \<Rightarrow> u64 option" where
-  "u64_mul \<equiv> check_bin_op u64_to_nat u64 any_args valid_u64 (*)"
-
-definition u64_div :: "u64 \<Rightarrow> u64 \<Rightarrow> u64 option" where
-  "u64_div \<equiv> check_bin_op u64_to_nat u64 (\<lambda>_ y. y \<noteq> u64 0) valid_u64 (div)"
-
-definition u64_mod :: "u64 \<Rightarrow> u64 \<Rightarrow> u64 option" where
-  "u64_mod \<equiv> check_bin_op u64_to_nat u64 (\<lambda>_ y. y \<noteq> u64 0) valid_u64 (mod)"
-
-definition lift_slot_bin_op :: "(u64 \<Rightarrow> u64 \<Rightarrow> u64 option) \<Rightarrow> Slot \<Rightarrow> Slot \<Rightarrow> Slot option" where
-  "lift_slot_bin_op \<equiv> check_bin_op_then slot_to_u64 Slot any_args valid_slot"
-
-definition lift_epoch_bin_op :: "(u64 \<Rightarrow> u64 \<Rightarrow> u64 option) \<Rightarrow> Epoch \<Rightarrow> Epoch \<Rightarrow> Epoch option" where
-  "lift_epoch_bin_op \<equiv> check_bin_op_then epoch_to_u64 Epoch any_args valid_epoch"
-
-definition slot_add :: "Slot \<Rightarrow> Slot \<Rightarrow> Slot option" where
-  "slot_add \<equiv> lift_slot_bin_op u64_add"
-
-definition slot_sub :: "Slot \<Rightarrow> Slot \<Rightarrow> Slot option" where
-  "slot_sub \<equiv> lift_slot_bin_op u64_sub"
-
-definition slot_mul :: "Slot \<Rightarrow> Slot \<Rightarrow> Slot option" where
-  "slot_mul \<equiv> lift_slot_bin_op u64_mul"
-
-definition slot_div :: "Slot \<Rightarrow> Slot \<Rightarrow> Slot option" where
-  "slot_div \<equiv> lift_slot_bin_op u64_div"
-
-definition slot_mod :: "Slot \<Rightarrow> Slot \<Rightarrow> Slot option" where
-  "slot_mod \<equiv> lift_slot_bin_op u64_mod"
-
-definition epoch_add :: "Epoch \<Rightarrow> Epoch \<Rightarrow> Epoch option" where
-  "epoch_add \<equiv> lift_epoch_bin_op u64_add"
-
-definition epoch_sub :: "Epoch \<Rightarrow> Epoch \<Rightarrow> Epoch option" where
-  "epoch_sub \<equiv> lift_epoch_bin_op u64_sub"
-
-definition epoch_mul :: "Epoch \<Rightarrow> Epoch \<Rightarrow> Epoch option" where
-  "epoch_mul \<equiv> lift_epoch_bin_op u64_mul"
-
-definition epoch_div :: "Epoch \<Rightarrow> Epoch \<Rightarrow> Epoch option" where
-  "epoch_div \<equiv> lift_epoch_bin_op u64_div"
-
-definition epoch_mod :: "Epoch \<Rightarrow> Epoch \<Rightarrow> Epoch option" where
-  "epoch_mod \<equiv> lift_epoch_bin_op u64_mod"
-
-adhoc_overloading
-  unsigned_add u64_add slot_add epoch_add and
-  unsigned_sub u64_sub slot_sub epoch_sub and
-  unsigned_mul u64_mul slot_mul epoch_mul and
-  unsigned_div u64_div slot_div epoch_div and
-  unsigned_mod u64_mod slot_mod epoch_mod
-
-lemmas u64_simps = valid_u64_def u64_add_def u64_sub_def u64_mul_def u64_div_def u64_mod_def
-lemmas slot_simps = valid_slot_def slot_add_def slot_sub_def slot_mul_def slot_div_def slot_mod_def
-                    lift_slot_bin_op_def
-lemmas epoch_simps = valid_epoch_def epoch_add_def epoch_sub_def epoch_mul_def epoch_div_def
-                     epoch_mod_def lift_epoch_bin_op_def
-lemmas unsigned_simps = any_args_def check_bin_op_then_def check_bin_op_def
-
-(* Sanity check lemmas *)
-lemma u64_add_overflow_int_max: "u64 (2 ^ 64 - 1) .+ u64 1 = None"
-  by (clarsimp simp: u64_simps unsigned_simps)
-
-lemma u64_add_overflow_contradiction: "(u64 (2 ^ 64 - 1) .+ u64 1 = Some (u64 0)) \<Longrightarrow> False"
-  by (clarsimp simp: u64_simps unsigned_simps)
-
-lemma u64_sub_overflow_zero: "u64 0 .- u64 1 = None"
-  by (clarsimp simp: u64_simps unsigned_simps)
-
-lemma u64_div_zero: "n \\ u64 0 = None"
-  by (clarsimp simp: u64_simps unsigned_simps)
-
-lemma slot_div_zero: "n \\ Slot (u64 0) = None"
-  by (clarsimp simp: slot_simps u64_simps unsigned_simps)
-
-lemma epoch_leq: "Epoch (u64 n) \<le> (Epoch (u64 (n + 1)))"
-  by (clarsimp simp: less_eq_Epoch_def less_eq_u64_def)
 
 end
